Use h_exists for lockinv instead of h_or

ulib/experimental/Steel.SpinLock.fst
@@ -9,8 +9,8 @@ let available = false
 let locked = true
 
 let lockinv (p:hprop) (r:ref bool) : hprop =
-  // h_exists (fun b -> pts_to r full_permission b `star` (if b then emp else p))
-  h_or (pts_to r full_permission available `star` p) (pts_to r full_permission locked `star` emp)
+  h_exists (fun b -> pts_to r full_permission (Ghost.hide b) `star` (if b then emp else p))
+//  h_or (pts_to r full_permission available `star` p) (pts_to r full_permission locked `star` emp)
 
 let lock (p:hprop) = (r:ref bool) & inv (lockinv p r)
 
@@ -51,32 +51,25 @@ assume
 val h_commute (#uses:Set.set lock_addr) (p q:hprop)
   : SteelAtomic unit uses true (p `star` q) (fun _ -> q `star` p)
 
-
 assume
-val intro_h_or_left (#uses:Set.set lock_addr) (p:hprop) (q:hprop)
-  : SteelAtomic unit uses true p (fun _ -> h_or p q)
+val intro_h_exists (#a:Type) (#uses:Set.set lock_addr) (x:a) (p:a -> hprop)
+  : SteelAtomic unit uses true (p x) (fun _ -> h_exists p)
 
-assume
-val intro_h_or_right (#uses:Set.set lock_addr) (p:hprop) (q:hprop)
-  : SteelAtomic unit uses true q (fun _ -> h_or p q)
-
-val intro_lockinv_left (#uses:Set.set lock_addr) (p:hprop) (r:ref bool)
+val intro_lockinv_available (#uses:Set.set lock_addr) (p:hprop) (r:ref bool)
   : SteelAtomic unit uses true (pts_to r full_permission available `star` p) (fun _ -> lockinv p r)
 
-val intro_lockinv_right (#uses:Set.set lock_addr) (p:hprop) (r:ref bool)
+val intro_lockinv_locked (#uses:Set.set lock_addr) (p:hprop) (r:ref bool)
   : SteelAtomic unit uses true (pts_to r full_permission locked) (fun _ -> lockinv p r)
 
-let intro_lockinv_left #uses p r =
-  intro_h_or_left
-    (pts_to r full_permission available `star` p)
-    (pts_to r full_permission locked `star` emp)
+let intro_lockinv_available #uses p r =
+  intro_h_exists false
+    (fun b -> pts_to r full_permission (Ghost.hide b) `star` (if b then emp else p))
 
-let intro_lockinv_right #uses p r =
+let intro_lockinv_locked #uses p r =
   h_intro_emp_l (pts_to r full_permission locked);
   h_commute emp (pts_to r full_permission locked);
-  intro_h_or_right
-    (pts_to r full_permission available `star` p)
-    (pts_to r full_permission locked `star` emp)
+  intro_h_exists true
+    (fun b -> pts_to r full_permission (Ghost.hide b) `star` (if b then emp else p))
 
 assume
 val lift_atomic_to_steelT
@@ -91,7 +84,7 @@ let new_lock (p:hprop)
   : SteelT (lock p) p (fun _ -> emp) =
   let r:ref bool =
     steel_frame_t (fun _ -> alloc available) in
-  lift_atomic_to_steelT (fun _ -> intro_lockinv_left p r);
+  lift_atomic_to_steelT (fun _ -> intro_lockinv_available p r);
   let i:inv (lockinv p r) = new_inv (lockinv p r) in
   let l:lock p = (| r, i |) in
   l
@@ -105,11 +98,11 @@ val ghost_read (#a:Type) (#uses:Set.set lock_addr) (#p:perm) (#v:Ghost.erased a)
 
 /// A specialized version of get_ref_refine. It should be derivable from h_exists
 assume
-val ghost_read_or (#uses:Set.set lock_addr) (#p:perm) (r:ref bool)
-  (q:bool -> hprop)
-  : SteelAtomic bool uses true
-    (h_or (pts_to r p false `star` q false) (pts_to r p true `star` q true))
-    (fun x -> pts_to r p x `star` q x)
+val ghost_read_refine (#a:Type) (#uses:Set.set lock_addr) (#p:perm) (r:ref a)
+  (q:a -> hprop)
+  : SteelAtomic a uses true
+    (h_exists (fun (v:a) -> pts_to r p v `star` q v))
+    (fun v -> pts_to r p v `star` q v)
 
 assume
 val cas
@@ -161,13 +154,13 @@ val acquire_core (#p:hprop) (#u:Set.set lock_addr) (r:ref bool) (i:inv (lockinv 
 let acquire_core #p #u r i =
   h_commute (lockinv p r) emp;
   h_elim_emp_l (lockinv p r);
-  let ghost = ghost_read_or r (fun b -> if b then emp else p) in
+  let ghost = ghost_read_refine r (fun b -> if b then emp else p) in
 
   let frame = if ghost then emp else p in
 
   let res = cas_frame r ghost available locked frame in
 
-  atomic_frame (if ghost then emp else p) (fun _ -> intro_lockinv_right p r);
+  atomic_frame (if ghost then emp else p) (fun _ -> intro_lockinv_locked p r);
 
   return_atomic #_ #_ #(fun b -> lockinv p r `star` (if b then p else emp)) res
 
@@ -198,7 +191,7 @@ let release_core #p #u r i =
   let v:bool = atomic_frame p (fun _ -> ghost_read r) in
   let res = cas_frame r v locked available p in
   h_assert_atomic (pts_to r full_permission available `star` p);
-  intro_lockinv_left p r;
+  intro_lockinv_available p r;
   h_intro_emp_l (lockinv p r);
   h_commute emp (lockinv p r)
 
